Refactor ArStepStar to use generic StepStar abstraction
Replace manual ArStepStar definition with reuse of the new generic
StepStar inductive type, and update proofs accordingly. Remove
unnecessary whitespace and fix naming inconsistencies.

ExprEval/Arithmetic.lean
@@ -1,6 +1,5 @@
 import ExprEval.Expr
 
-
 variable (V: Type)
 
 -- Arithmetic Expressions
@@ -48,6 +47,6 @@ inductive ArStep: (val: V -> Int) -> (ArExpr V) -> (ArExpr V) -> Prop where
     | subRight (n: Int) (e₂ e₂': ArExpr V) : ArStep val e₂ e₂' -> ArStep val (ArExpr.Sub (ArExpr.Const n) e₂)  (ArExpr.Sub (ArExpr.Const n) e₂')
     | mulRight (n: Int) (e₂ e₂': ArExpr V) : ArStep val e₂ e₂' -> ArStep val (ArExpr.Mul (ArExpr.Const n) e₂)  (ArExpr.Mul (ArExpr.Const n) e₂')
 
-inductive ArStepStar : (val: V -> Int) -> (ArExpr V) -> (ArExpr V) -> Prop where
-    | refl val e : ArStepStar val e e
-    | trans e₁ e₂ e₃ : (ArStep V val) e₁ e₂ -> ArStepStar val e₂ e₃ -> ArStepStar val e₁ e₃
+def ArStepStar (V: Type) := StepStar (StepKind := ArStep V) V
+def ArStepStar.refl {V: Type} (val: V -> Int) := StepStar.refl (StepKind := ArStep V) val
+def ArStepStar.trans {V: Type} {val: V -> Int} e₁ e₂ e₃ := StepStar.trans e₁ e₂ e₃ (StepKind := ArStep V) (val := val)
